lean/Pcc116/Aula03.lean
@@ -1,0 +1,161 @@
+
+import Mathlib.Data.Int.Basic
+import Mathlib.Data.Nat.Basic
+import Mathlib.Data.List.Basic 
+
+-- inversão de listas 
+
+def reverse {α : Type} : List α → List α
+  | []      => []
+  | x :: xs => reverse xs ++ [x]
+
+lemma reverse_cat {a : Type} 
+   (xs ys : List a) 
+  : reverse (xs ++ ys) = 
+    reverse ys ++ reverse xs := by 
+    induction xs with 
+    | nil =>
+      simp [reverse] 
+    | cons x xs IHxs => 
+      simp [reverse, IHxs, List.append_assoc]
+
+theorem reverse_reverse {α : Type} 
+    (xs : List α) :
+    reverse (reverse xs) = xs := by 
+  induction xs with 
+  | nil => simp [reverse] 
+  | cons y ys IHys => 
+    simp [reverse, IHys, reverse_cat]
+
+-- otimizando a inversão usando acumulador
+
+def rev_acc {a : Type} 
+  : List a -> List a -> List a 
+| [], ac => ac 
+| x :: xs, ac => rev_acc xs (x :: ac)
+
+def rev {a : Type} (xs : List a) : List a := 
+  rev_acc xs []
+
+-- provando a equivalência das def. 
+
+lemma rev_acc_append {a : Type} 
+  (xs ys zs : List a) 
+  : rev_acc xs ys ++ zs = rev_acc xs (ys ++ zs) 
+    := by 
+    revert ys zs 
+    induction xs with 
+    | nil => 
+      simp [rev_acc]
+    | cons x1 xs1 IHxs1 =>
+      intros ys zs 
+      simp [rev_acc, IHxs1]
+
+theorem reverse_rev {a : Type}
+  (xs : List a) : rev xs = reverse xs := by
+  induction xs with 
+  | nil =>
+    simp [rev, rev_acc, reverse]
+  | cons y ys IHys => 
+    simp [rev, rev_acc, reverse, <- IHys, rev_acc_append] 
+    
+-- map and foldr 
+
+def map {a b : Type} (f : a -> b) 
+  : List a -> List b 
+| [] => [] 
+| x :: xs => f x :: map f xs 
+
+def foldr {a b : Type}(f : a -> b -> b)(v : b) 
+  : List a -> b 
+| [] => v 
+| x :: xs => f x (foldr f v xs) 
+
+-- id x = x
+
+theorem map_id {a : Type} (xs : List a) 
+  : map id xs = xs := by 
+  induction xs with 
+  | nil => simp [map]
+  | cons y ys IHys => 
+    simp [map, IHys]
+
+theorem map_append {a b : Type} 
+  (f : a -> b)(xs ys : List a) : 
+  map f (xs ++ ys) = map f xs ++ map f ys := by 
+  induction xs with 
+  | nil => simp [map]
+  | cons x xs IHxs => 
+    simp [map]
+    exact IHxs  
+
+def compose {a b c : Type}
+  (g : b -> c)(f : a -> b) : a -> c := 
+    fun x => g (f x) 
+
+infixl:90 "•" => compose
+
+theorem map_fusion {a b c : Type}
+  (f : a -> b)(g : b -> c)(xs : List a) : 
+  map (g • f) xs = map g (map f xs) := by 
+    induction xs with 
+    | nil => 
+      simp [map]
+    | cons x xs IHxs =>
+      simp [map, IHxs, compose]
+
+theorem foldr_map_fusion {a b c : Type}
+  (f : a -> b)(g : b -> c -> c)
+  (v : c)(xs : List a) 
+  : (foldr g v • map f) xs = foldr (g • f) v xs 
+    := by
+    induction xs with 
+    | nil =>
+      simp [foldr, map, compose]
+    | cons x xs IHxs => 
+      simp [compose, map, foldr]
+      rw [<- IHxs] 
+      simp [compose] 
+
+-- árvores binárias 
+
+inductive BTree (a : Type) : Type where 
+| Leaf : BTree a 
+| Node : a -> BTree a -> BTree a -> BTree a 
+
+def BTree.size {a : Type} : BTree a -> ℕ 
+| .Leaf => 0 
+| .Node _ l r => l.size + r.size + 1 
+
+def BTree.height {a :Type} : BTree a -> ℕ 
+| .Leaf => 0 
+| .Node _ l r => 1 + (max l.height r.height)
+  
+
+theorem BTree.height_le_size {a : Type}
+  (t : BTree a) : t.height <= t.size := by
+  induction t with 
+  | Leaf =>
+    simp [size, height]
+  | Node x l r IHl IHr =>
+    simp [size, height] 
+    simp [max] 
+    split_ifs 
+    · 
+      rw [Nat.add_comm _ r.height]
+      simp 
+      omega 
+    · 
+      rw [Nat.add_comm _ l.height] 
+      simp 
+      omega 
+
+def BTree.mirror {a : Type} : BTree a -> BTree a 
+| .Leaf => .Leaf 
+| .Node x l r => .Node x r.mirror l.mirror
+
+theorem BTree.mirror_mirror {a : Type}
+  (t : BTree a) : t.mirror.mirror = t := by 
+  sorry 
+
+
