listas/lista02/Lista02.lean
@@ -1,0 +1,1 @@
+import Lista02.Basic
